WIP: stutter to ksim

src/ModSimStutter.v
@@ -40,10 +40,9 @@ Section PRIMIVIESIM.
   Variable I: shared_rel.
 
   Variant __lsim
-          (tid: thread_id)
-          (lsim: forall R_src R_tgt (RR: R_src -> R_tgt -> URA.car -> shared_rel), bool -> bool -> URA.car -> ((wf_stt R_src R_tgt).(T) * itree srcE R_src) -> itree tgtE R_tgt -> shared_rel)
-          (_lsim: forall R_src R_tgt (RR: R_src -> R_tgt -> URA.car -> shared_rel),bool -> bool -> URA.car -> ((wf_stt R_src R_tgt).(T) * itree srcE R_src) -> itree tgtE R_tgt -> shared_rel)
-          R_src R_tgt (RR: R_src -> R_tgt -> URA.car -> shared_rel)
+          (tid: thread_id) R_src R_tgt (RR: R_src -> R_tgt -> URA.car -> shared_rel)
+          (lsim: bool -> bool -> URA.car -> ((wf_stt R_src R_tgt).(T) * itree srcE R_src) -> itree tgtE R_tgt -> shared_rel)
+          (_lsim: bool -> bool -> URA.car -> ((wf_stt R_src R_tgt).(T) * itree srcE R_src) -> itree tgtE R_tgt -> shared_rel)
     :
     bool -> bool -> URA.car -> ((wf_stt R_src R_tgt).(T) * itree srcE R_src) -> itree tgtE R_tgt -> shared_rel :=
   | lsim_ret
@@ -53,112 +52,112 @@ Section PRIMIVIESIM.
       (LT: (wf_stt R_src R_tgt).(lt) o0 o)
       (LSIM: RR r_src r_tgt r_ctx (ths, im_src, im_tgt, st_src, st_tgt, r_shared))
     :
-    __lsim tid lsim _lsim RR f_src f_tgt r_ctx (o, Ret r_src) (Ret r_tgt) (ths, im_src, im_tgt, st_src, st_tgt, r_shared)
+    __lsim tid RR lsim _lsim f_src f_tgt r_ctx (o, Ret r_src) (Ret r_tgt) (ths, im_src, im_tgt, st_src, st_tgt, r_shared)
 
   | lsim_tauL
       f_src f_tgt r_ctx o
       ths im_src im_tgt st_src st_tgt r_shared
       itr_src itr_tgt
-      (LSIM: _lsim _ _ RR true f_tgt r_ctx (o, itr_src) itr_tgt (ths, im_src, im_tgt, st_src, st_tgt, r_shared))
+      (LSIM: _lsim true f_tgt r_ctx (o, itr_src) itr_tgt (ths, im_src, im_tgt, st_src, st_tgt, r_shared))
     :
-    __lsim tid lsim _lsim RR f_src f_tgt r_ctx (o, Tau itr_src) itr_tgt (ths, im_src, im_tgt, st_src, st_tgt, r_shared)
+    __lsim tid RR lsim _lsim f_src f_tgt r_ctx (o, Tau itr_src) itr_tgt (ths, im_src, im_tgt, st_src, st_tgt, r_shared)
   | lsim_chooseL
       f_src f_tgt r_ctx o
       ths im_src im_tgt st_src st_tgt r_shared
       X ktr_src itr_tgt
-      (LSIM: exists x, _lsim _ _ RR true f_tgt r_ctx (o, ktr_src x) itr_tgt (ths, im_src, im_tgt, st_src, st_tgt, r_shared))
+      (LSIM: exists x, _lsim true f_tgt r_ctx (o, ktr_src x) itr_tgt (ths, im_src, im_tgt, st_src, st_tgt, r_shared))
     :
-    __lsim tid lsim _lsim RR f_src f_tgt r_ctx (o, trigger (Choose X) >>= ktr_src) itr_tgt (ths, im_src, im_tgt, st_src, st_tgt, r_shared)
+    __lsim tid RR lsim _lsim f_src f_tgt r_ctx (o, trigger (Choose X) >>= ktr_src) itr_tgt (ths, im_src, im_tgt, st_src, st_tgt, r_shared)
   | lsim_putL
       f_src f_tgt r_ctx o
       ths im_src im_tgt st_src st_tgt r_shared
       st ktr_src itr_tgt
-      (LSIM: _lsim _ _ RR true f_tgt r_ctx (o, ktr_src tt) itr_tgt (ths, im_src, im_tgt, st, st_tgt, r_shared))
+      (LSIM: _lsim true f_tgt r_ctx (o, ktr_src tt) itr_tgt (ths, im_src, im_tgt, st, st_tgt, r_shared))
     :
-    __lsim tid lsim _lsim RR f_src f_tgt r_ctx (o, trigger (Put st) >>= ktr_src) itr_tgt (ths, im_src, im_tgt, st_src, st_tgt, r_shared)
+    __lsim tid RR lsim _lsim f_src f_tgt r_ctx (o, trigger (Put st) >>= ktr_src) itr_tgt (ths, im_src, im_tgt, st_src, st_tgt, r_shared)
   | lsim_getL
       f_src f_tgt r_ctx o
       ths im_src im_tgt st_src st_tgt r_shared
       ktr_src itr_tgt
-      (LSIM: _lsim _ _ RR true f_tgt r_ctx (o, ktr_src st_src) itr_tgt (ths, im_src, im_tgt, st_src, st_tgt, r_shared))
+      (LSIM: _lsim true f_tgt r_ctx (o, ktr_src st_src) itr_tgt (ths, im_src, im_tgt, st_src, st_tgt, r_shared))
     :
-    __lsim tid lsim _lsim RR f_src f_tgt r_ctx (o, trigger (@Get _) >>= ktr_src) itr_tgt (ths, im_src, im_tgt, st_src, st_tgt, r_shared)
+    __lsim tid RR lsim _lsim f_src f_tgt r_ctx (o, trigger (@Get _) >>= ktr_src) itr_tgt (ths, im_src, im_tgt, st_src, st_tgt, r_shared)
   | lsim_tidL
       f_src f_tgt r_ctx o
       ths im_src im_tgt st_src st_tgt r_shared
       ktr_src itr_tgt
-      (LSIM: _lsim _ _ RR true f_tgt r_ctx (o, ktr_src tid) itr_tgt (ths, im_src, im_tgt, st_src, st_tgt, r_shared))
+      (LSIM: _lsim true f_tgt r_ctx (o, ktr_src tid) itr_tgt (ths, im_src, im_tgt, st_src, st_tgt, r_shared))
     :
-    __lsim tid lsim _lsim RR f_src f_tgt r_ctx (o, trigger (GetTid) >>= ktr_src) itr_tgt (ths, im_src, im_tgt, st_src, st_tgt, r_shared)
+    __lsim tid RR lsim _lsim f_src f_tgt r_ctx (o, trigger (GetTid) >>= ktr_src) itr_tgt (ths, im_src, im_tgt, st_src, st_tgt, r_shared)
   | lsim_UB
       f_src f_tgt r_ctx o
       ths im_src im_tgt st_src st_tgt r_shared
       ktr_src itr_tgt
     :
-    __lsim tid lsim _lsim RR f_src f_tgt r_ctx (o, trigger (Undefined) >>= ktr_src) itr_tgt (ths, im_src, im_tgt, st_src, st_tgt, r_shared)
+    __lsim tid RR lsim _lsim f_src f_tgt r_ctx (o, trigger (Undefined) >>= ktr_src) itr_tgt (ths, im_src, im_tgt, st_src, st_tgt, r_shared)
   | lsim_fairL
       f_src f_tgt r_ctx o
       ths im_src0 im_tgt st_src st_tgt r_shared
       f ktr_src itr_tgt
       (LSIM: exists im_src1,
           (<<FAIR: fair_update im_src0 im_src1 (sum_fmap_r f)>>) /\
-            (<<LSIM: _lsim _ _ RR true f_tgt r_ctx (o, ktr_src tt) itr_tgt (ths, im_src1, im_tgt, st_src, st_tgt, r_shared)>>))
+            (<<LSIM: _lsim true f_tgt r_ctx (o, ktr_src tt) itr_tgt (ths, im_src1, im_tgt, st_src, st_tgt, r_shared)>>))
     :
-    __lsim tid lsim _lsim RR f_src f_tgt r_ctx (o, trigger (Fair f) >>= ktr_src) itr_tgt (ths, im_src0, im_tgt, st_src, st_tgt, r_shared)
+    __lsim tid RR lsim _lsim f_src f_tgt r_ctx (o, trigger (Fair f) >>= ktr_src) itr_tgt (ths, im_src0, im_tgt, st_src, st_tgt, r_shared)
 
   | lsim_tauR
       f_src f_tgt r_ctx o
       ths im_src im_tgt st_src st_tgt r_shared
       itr_src itr_tgt
-      (LSIM: _lsim _ _ RR f_src true r_ctx (o, itr_src) itr_tgt (ths, im_src, im_tgt, st_src, st_tgt, r_shared))
+      (LSIM: _lsim f_src true r_ctx (o, itr_src) itr_tgt (ths, im_src, im_tgt, st_src, st_tgt, r_shared))
     :
-    __lsim tid lsim _lsim RR f_src f_tgt r_ctx (o, itr_src) (Tau itr_tgt) (ths, im_src, im_tgt, st_src, st_tgt, r_shared)
+    __lsim tid RR lsim _lsim f_src f_tgt r_ctx (o, itr_src) (Tau itr_tgt) (ths, im_src, im_tgt, st_src, st_tgt, r_shared)
   | lsim_chooseR
       f_src f_tgt r_ctx o
       ths im_src im_tgt st_src st_tgt r_shared
       X itr_src ktr_tgt
-      (LSIM: forall x, _lsim _ _ RR f_src true r_ctx (o, itr_src) (ktr_tgt x) (ths, im_src, im_tgt, st_src, st_tgt, r_shared))
+      (LSIM: forall x, _lsim f_src true r_ctx (o, itr_src) (ktr_tgt x) (ths, im_src, im_tgt, st_src, st_tgt, r_shared))
     :
-    __lsim tid lsim _lsim RR f_src f_tgt r_ctx (o, itr_src) (trigger (Choose X) >>= ktr_tgt) (ths, im_src, im_tgt, st_src, st_tgt, r_shared)
+    __lsim tid RR lsim _lsim f_src f_tgt r_ctx (o, itr_src) (trigger (Choose X) >>= ktr_tgt) (ths, im_src, im_tgt, st_src, st_tgt, r_shared)
   | lsim_putR
       f_src f_tgt r_ctx o
       ths im_src im_tgt st_src st_tgt r_shared
       st itr_src ktr_tgt
-      (LSIM: _lsim _ _ RR f_src true r_ctx (o, itr_src) (ktr_tgt tt) (ths, im_src, im_tgt, st_src, st, r_shared))
+      (LSIM: _lsim f_src true r_ctx (o, itr_src) (ktr_tgt tt) (ths, im_src, im_tgt, st_src, st, r_shared))
     :
-    __lsim tid lsim _lsim RR f_src f_tgt r_ctx (o, itr_src) (trigger (Put st) >>= ktr_tgt) (ths, im_src, im_tgt, st_src, st_tgt, r_shared)
+    __lsim tid RR lsim _lsim f_src f_tgt r_ctx (o, itr_src) (trigger (Put st) >>= ktr_tgt) (ths, im_src, im_tgt, st_src, st_tgt, r_shared)
   | lsim_getR
       f_src f_tgt r_ctx o
       ths im_src im_tgt st_src st_tgt r_shared
       itr_src ktr_tgt
-      (LSIM: _lsim _ _ RR f_src true r_ctx (o, itr_src) (ktr_tgt st_tgt) (ths, im_src, im_tgt, st_src, st_tgt, r_shared))
+      (LSIM: _lsim f_src true r_ctx (o, itr_src) (ktr_tgt st_tgt) (ths, im_src, im_tgt, st_src, st_tgt, r_shared))
     :
-    __lsim tid lsim _lsim RR f_src f_tgt r_ctx (o, itr_src) (trigger (@Get _) >>= ktr_tgt) (ths, im_src, im_tgt, st_src, st_tgt, r_shared)
+    __lsim tid RR lsim _lsim f_src f_tgt r_ctx (o, itr_src) (trigger (@Get _) >>= ktr_tgt) (ths, im_src, im_tgt, st_src, st_tgt, r_shared)
   | lsim_tidR
       f_src f_tgt r_ctx o
       ths im_src im_tgt st_src st_tgt r_shared
       itr_src ktr_tgt
-      (LSIM: _lsim _ _ RR f_src true r_ctx (o, itr_src) (ktr_tgt tid) (ths, im_src, im_tgt, st_src, st_tgt, r_shared))
+      (LSIM: _lsim f_src true r_ctx (o, itr_src) (ktr_tgt tid) (ths, im_src, im_tgt, st_src, st_tgt, r_shared))
     :
-    __lsim tid lsim _lsim RR f_src f_tgt r_ctx (o, itr_src) (trigger (GetTid) >>= ktr_tgt) (ths, im_src, im_tgt, st_src, st_tgt, r_shared)
+    __lsim tid RR lsim _lsim f_src f_tgt r_ctx (o, itr_src) (trigger (GetTid) >>= ktr_tgt) (ths, im_src, im_tgt, st_src, st_tgt, r_shared)
   | lsim_fairR
       f_src f_tgt r_ctx o
       ths im_src im_tgt0 st_src st_tgt r_shared
       f itr_src ktr_tgt
       (LSIM: forall im_tgt1
                    (FAIR: fair_update im_tgt0 im_tgt1 (sum_fmap_r f)),
-          (<<LSIM: _lsim _ _ RR f_src true r_ctx (o, itr_src) (ktr_tgt tt) (ths, im_src, im_tgt1, st_src, st_tgt, r_shared)>>))
+          (<<LSIM: _lsim f_src true r_ctx (o, itr_src) (ktr_tgt tt) (ths, im_src, im_tgt1, st_src, st_tgt, r_shared)>>))
     :
-    __lsim tid lsim _lsim RR f_src f_tgt r_ctx (o, itr_src) (trigger (Fair f) >>= ktr_tgt) (ths, im_src, im_tgt0, st_src, st_tgt, r_shared)
+    __lsim tid RR lsim _lsim f_src f_tgt r_ctx (o, itr_src) (trigger (Fair f) >>= ktr_tgt) (ths, im_src, im_tgt0, st_src, st_tgt, r_shared)
 
   | lsim_observe
       f_src f_tgt r_ctx o
       ths im_src im_tgt st_src st_tgt r_shared
       fn args ktr_src ktr_tgt
       (LSIM: forall ret,
-          lsim _ _ RR true true r_ctx (o, ktr_src ret) (ktr_tgt ret) (ths, im_src, im_tgt, st_src, st_tgt, r_shared))
+          lsim true true r_ctx (o, ktr_src ret) (ktr_tgt ret) (ths, im_src, im_tgt, st_src, st_tgt, r_shared))
     :
-    __lsim tid lsim _lsim RR f_src f_tgt r_ctx (o, trigger (Observe fn args) >>= ktr_src) (trigger (Observe fn args) >>= ktr_tgt) (ths, im_src, im_tgt, st_src, st_tgt, r_shared)
+    __lsim tid RR lsim _lsim f_src f_tgt r_ctx (o, trigger (Observe fn args) >>= ktr_src) (trigger (Observe fn args) >>= ktr_tgt) (ths, im_src, im_tgt, st_src, st_tgt, r_shared)
 
   | lsim_yieldR
       f_src f_tgt r_ctx0 o0
@@ -173,42 +172,42 @@ Section PRIMIVIESIM.
                im_tgt2
                (TGT: fair_update im_tgt1 im_tgt2 (sum_fmap_l (tids_fmap tid ths1))),
         exists o1,
-            (<<LSIM: lsim _ _ RR true true r_ctx1 (o1, trigger (Yield) >>= ktr_src) (ktr_tgt tt) (ths1, im_src1, im_tgt2, st_src1, st_tgt1, r_shared1)>>) /\
+            (<<LSIM: lsim true true r_ctx1 (o1, trigger (Yield) >>= ktr_src) (ktr_tgt tt) (ths1, im_src1, im_tgt2, st_src1, st_tgt1, r_shared1)>>) /\
               (<<STUTTER: (wf_stt R_src R_tgt).(lt) o1 o0>>))
     :
-    __lsim tid lsim _lsim RR f_src f_tgt r_ctx0 (o0, trigger (Yield) >>= ktr_src) (trigger (Yield) >>= ktr_tgt) (ths0, im_src0, im_tgt0, st_src0, st_tgt0, r_shared0)
+    __lsim tid RR lsim _lsim f_src f_tgt r_ctx0 (o0, trigger (Yield) >>= ktr_src) (trigger (Yield) >>= ktr_tgt) (ths0, im_src0, im_tgt0, st_src0, st_tgt0, r_shared0)
   | lsim_yieldL
       f_src f_tgt r_ctx o0
       ths im_src0 im_tgt st_src st_tgt r_shared
       ktr_src itr_tgt
       (LSIM: exists im_src1 o1,
           (<<FAIR: fair_update im_src0 im_src1 (sum_fmap_l (tids_fmap tid ths))>>) /\
-            (<<LSIM: _lsim _ _ RR true f_tgt r_ctx (o1, ktr_src tt) itr_tgt (ths, im_src1, im_tgt, st_src, st_tgt, r_shared)>>))
+            (<<LSIM: _lsim true f_tgt r_ctx (o1, ktr_src tt) itr_tgt (ths, im_src1, im_tgt, st_src, st_tgt, r_shared)>>))
     :
-    __lsim tid lsim _lsim RR f_src f_tgt r_ctx (o0, trigger (Yield) >>= ktr_src) itr_tgt (ths, im_src0, im_tgt, st_src, st_tgt, r_shared)
+    __lsim tid RR lsim _lsim f_src f_tgt r_ctx (o0, trigger (Yield) >>= ktr_src) itr_tgt (ths, im_src0, im_tgt, st_src, st_tgt, r_shared)
 
   | lsim_progress
       r_ctx o
       ths im_src im_tgt st_src st_tgt r_shared
       itr_src itr_tgt
-      (LSIM: lsim _ _ RR false false r_ctx (o, itr_src) itr_tgt (ths, im_src, im_tgt, st_src, st_tgt, r_shared))
+      (LSIM: lsim false false r_ctx (o, itr_src) itr_tgt (ths, im_src, im_tgt, st_src, st_tgt, r_shared))
     :
-    __lsim tid lsim _lsim RR true true r_ctx (o, itr_src) itr_tgt (ths, im_src, im_tgt, st_src, st_tgt, r_shared)
+    __lsim tid RR lsim _lsim true true r_ctx (o, itr_src) itr_tgt (ths, im_src, im_tgt, st_src, st_tgt, r_shared)
   .
 
   Definition lsim (tid: thread_id)
              R_src R_tgt (RR: R_src -> R_tgt -> URA.car -> shared_rel):
     bool -> bool -> URA.car -> ((wf_stt R_src R_tgt).(T) * itree srcE R_src) -> itree tgtE R_tgt -> shared_rel :=
-    paco9 (fun r => pind9 (__lsim tid r) top9) bot9 R_src R_tgt RR.
+    paco6 (fun r => pind6 (__lsim tid RR r) top6) bot6.
 
-  Lemma __lsim_mon tid:
-    forall r r' (LE: r <9= r'), (__lsim tid r) <10= (__lsim tid r').
+  Lemma __lsim_mon tid R0 R1 (RR: R0 -> R1 -> _ -> _):
+    forall r r' (LE: r <6= r'), (__lsim tid RR r) <7= (__lsim tid RR r').
   Proof.
     ii. inv PR; try (econs; eauto; fail).
     eapply lsim_yieldR; eauto. i. hexploit LSIM; eauto. i. des. esplits; eauto.
   Qed.
 
-  Lemma _lsim_mon tid: forall r, monotone9 (__lsim tid r).
+  Lemma _lsim_mon tid R0 R1 (RR: R0 -> R1 -> _ -> _): forall r, monotone6 (__lsim tid RR r).
   Proof.
     ii. inv IN; try (econs; eauto; fail).
     { des. econs; eauto. }
@@ -217,15 +216,15 @@ Section PRIMIVIESIM.
     { des. econs; esplits; eauto. }
   Qed.
 
-  Lemma lsim_mon tid: forall q, monotone9 (fun r => pind9 (__lsim tid r) q).
+  Lemma lsim_mon tid R0 R1 (RR: R0 -> R1 -> _ -> _):
+    forall q, monotone6 (fun r => pind6 (__lsim tid RR r) q).
   Proof.
-    ii. eapply pind9_mon_gen; eauto.
+    ii. eapply pind6_mon_gen; eauto.
     ii. eapply __lsim_mon; eauto.
   Qed.
 
-  Variant lsim_indC tid
-          (r: forall R_src R_tgt (RR: R_src -> R_tgt -> URA.car -> shared_rel), bool -> bool -> URA.car -> ((wf_stt R_src R_tgt).(T) * itree srcE R_src) -> itree tgtE R_tgt -> shared_rel)
-          R_src R_tgt (RR: R_src -> R_tgt -> URA.car -> shared_rel)
+  Variant lsim_indC tid R_src R_tgt (RR: R_src -> R_tgt -> URA.car -> shared_rel)
+          (r: bool -> bool -> URA.car -> ((wf_stt R_src R_tgt).(T) * itree srcE R_src) -> itree tgtE R_tgt -> shared_rel)
     :
     bool -> bool -> URA.car -> ((wf_stt R_src R_tgt).(T) * itree srcE R_src) -> itree tgtE R_tgt -> shared_rel :=
     | lsim_indC_ret
@@ -235,112 +234,112 @@ Section PRIMIVIESIM.
         (LT: (wf_stt R_src R_tgt).(lt) o0 o)
         (LSIM: RR r_src r_tgt r_ctx (ths, im_src, im_tgt, st_src, st_tgt, r_shared))
       :
-      lsim_indC tid r RR f_src f_tgt r_ctx (o, Ret r_src) (Ret r_tgt) (ths, im_src, im_tgt, st_src, st_tgt, r_shared)
+      lsim_indC tid RR r f_src f_tgt r_ctx (o, Ret r_src) (Ret r_tgt) (ths, im_src, im_tgt, st_src, st_tgt, r_shared)
 
     | lsim_indC_tauL
         f_src f_tgt r_ctx o
         ths im_src im_tgt st_src st_tgt r_shared
         itr_src itr_tgt
-        (LSIM: r _ _ RR true f_tgt r_ctx (o, itr_src) itr_tgt (ths, im_src, im_tgt, st_src, st_tgt, r_shared))
+        (LSIM: r true f_tgt r_ctx (o, itr_src) itr_tgt (ths, im_src, im_tgt, st_src, st_tgt, r_shared))
       :
-      lsim_indC tid r RR f_src f_tgt r_ctx (o, Tau itr_src) itr_tgt (ths, im_src, im_tgt, st_src, st_tgt, r_shared)
+      lsim_indC tid RR r f_src f_tgt r_ctx (o, Tau itr_src) itr_tgt (ths, im_src, im_tgt, st_src, st_tgt, r_shared)
     | lsim_indC_chooseL
         f_src f_tgt r_ctx o
         ths im_src im_tgt st_src st_tgt r_shared
         X ktr_src itr_tgt
-        (LSIM: exists x, r _ _ RR true f_tgt r_ctx (o, ktr_src x) itr_tgt (ths, im_src, im_tgt, st_src, st_tgt, r_shared))
+        (LSIM: exists x, r true f_tgt r_ctx (o, ktr_src x) itr_tgt (ths, im_src, im_tgt, st_src, st_tgt, r_shared))
       :
-      lsim_indC tid r RR f_src f_tgt r_ctx (o, trigger (Choose X) >>= ktr_src) itr_tgt (ths, im_src, im_tgt, st_src, st_tgt, r_shared)
+      lsim_indC tid RR r f_src f_tgt r_ctx (o, trigger (Choose X) >>= ktr_src) itr_tgt (ths, im_src, im_tgt, st_src, st_tgt, r_shared)
     | lsim_indC_putL
         f_src f_tgt r_ctx o
         ths im_src im_tgt st_src st_tgt r_shared
         st ktr_src itr_tgt
-        (LSIM: r _ _ RR true f_tgt r_ctx (o, ktr_src tt) itr_tgt (ths, im_src, im_tgt, st, st_tgt, r_shared))
+        (LSIM: r true f_tgt r_ctx (o, ktr_src tt) itr_tgt (ths, im_src, im_tgt, st, st_tgt, r_shared))
       :
-      lsim_indC tid r RR f_src f_tgt r_ctx (o, trigger (Put st) >>= ktr_src) itr_tgt (ths, im_src, im_tgt, st_src, st_tgt, r_shared)
+      lsim_indC tid RR r f_src f_tgt r_ctx (o, trigger (Put st) >>= ktr_src) itr_tgt (ths, im_src, im_tgt, st_src, st_tgt, r_shared)
     | lsim_indC_getL
         f_src f_tgt r_ctx o
         ths im_src im_tgt st_src st_tgt r_shared
         ktr_src itr_tgt
-        (LSIM: r _ _ RR true f_tgt r_ctx (o, ktr_src st_src) itr_tgt (ths, im_src, im_tgt, st_src, st_tgt, r_shared))
+        (LSIM: r true f_tgt r_ctx (o, ktr_src st_src) itr_tgt (ths, im_src, im_tgt, st_src, st_tgt, r_shared))
       :
-      lsim_indC tid r RR f_src f_tgt r_ctx (o, trigger (@Get _) >>= ktr_src) itr_tgt (ths, im_src, im_tgt, st_src, st_tgt, r_shared)
+      lsim_indC tid RR r f_src f_tgt r_ctx (o, trigger (@Get _) >>= ktr_src) itr_tgt (ths, im_src, im_tgt, st_src, st_tgt, r_shared)
     | lsim_indC_tidL
         f_src f_tgt r_ctx o
         ths im_src im_tgt st_src st_tgt r_shared
         ktr_src itr_tgt
-        (LSIM: r _ _ RR true f_tgt r_ctx (o, ktr_src tid) itr_tgt (ths, im_src, im_tgt, st_src, st_tgt, r_shared))
+        (LSIM: r true f_tgt r_ctx (o, ktr_src tid) itr_tgt (ths, im_src, im_tgt, st_src, st_tgt, r_shared))
       :
-      lsim_indC tid r RR f_src f_tgt r_ctx (o, trigger (GetTid) >>= ktr_src) itr_tgt (ths, im_src, im_tgt, st_src, st_tgt, r_shared)
+      lsim_indC tid RR r f_src f_tgt r_ctx (o, trigger (GetTid) >>= ktr_src) itr_tgt (ths, im_src, im_tgt, st_src, st_tgt, r_shared)
     | lsim_indC_UB
         f_src f_tgt r_ctx o
         ths im_src im_tgt st_src st_tgt r_shared
         ktr_src itr_tgt
       :
-      lsim_indC tid r RR f_src f_tgt r_ctx (o, trigger (Undefined) >>= ktr_src) itr_tgt (ths, im_src, im_tgt, st_src, st_tgt, r_shared)
+      lsim_indC tid RR r f_src f_tgt r_ctx (o, trigger (Undefined) >>= ktr_src) itr_tgt (ths, im_src, im_tgt, st_src, st_tgt, r_shared)
     | lsim_indC_fairL
         f_src f_tgt r_ctx o
         ths im_src0 im_tgt st_src st_tgt r_shared
         f ktr_src itr_tgt
         (LSIM: exists im_src1,
             (<<FAIR: fair_update im_src0 im_src1 (sum_fmap_r f)>>) /\
-              (<<LSIM: r _ _ RR true f_tgt r_ctx (o, ktr_src tt) itr_tgt (ths, im_src1, im_tgt, st_src, st_tgt, r_shared)>>))
+              (<<LSIM: r true f_tgt r_ctx (o, ktr_src tt) itr_tgt (ths, im_src1, im_tgt, st_src, st_tgt, r_shared)>>))
       :
-      lsim_indC tid r RR f_src f_tgt r_ctx (o, trigger (Fair f) >>= ktr_src) itr_tgt (ths, im_src0, im_tgt, st_src, st_tgt, r_shared)
+      lsim_indC tid RR r f_src f_tgt r_ctx (o, trigger (Fair f) >>= ktr_src) itr_tgt (ths, im_src0, im_tgt, st_src, st_tgt, r_shared)
 
     | lsim_indC_tauR
         f_src f_tgt r_ctx o
         ths im_src im_tgt st_src st_tgt r_shared
         itr_src itr_tgt
-        (LSIM: r _ _ RR f_src true r_ctx (o, itr_src) itr_tgt (ths, im_src, im_tgt, st_src, st_tgt, r_shared))
+        (LSIM: r f_src true r_ctx (o, itr_src) itr_tgt (ths, im_src, im_tgt, st_src, st_tgt, r_shared))
       :
-      lsim_indC tid r RR f_src f_tgt r_ctx (o, itr_src) (Tau itr_tgt) (ths, im_src, im_tgt, st_src, st_tgt, r_shared)
+      lsim_indC tid RR r f_src f_tgt r_ctx (o, itr_src) (Tau itr_tgt) (ths, im_src, im_tgt, st_src, st_tgt, r_shared)
     | lsim_indC_chooseR
         f_src f_tgt r_ctx o
         ths im_src im_tgt st_src st_tgt r_shared
         X itr_src ktr_tgt
-        (LSIM: forall x, r _ _ RR f_src true r_ctx (o, itr_src) (ktr_tgt x) (ths, im_src, im_tgt, st_src, st_tgt, r_shared))
+        (LSIM: forall x, r f_src true r_ctx (o, itr_src) (ktr_tgt x) (ths, im_src, im_tgt, st_src, st_tgt, r_shared))
       :
-      lsim_indC tid r RR f_src f_tgt r_ctx (o, itr_src) (trigger (Choose X) >>= ktr_tgt) (ths, im_src, im_tgt, st_src, st_tgt, r_shared)
+      lsim_indC tid RR r f_src f_tgt r_ctx (o, itr_src) (trigger (Choose X) >>= ktr_tgt) (ths, im_src, im_tgt, st_src, st_tgt, r_shared)
     | lsim_indC_putR
         f_src f_tgt r_ctx o
         ths im_src im_tgt st_src st_tgt r_shared
         st itr_src ktr_tgt
-        (LSIM: r _ _ RR f_src true r_ctx (o, itr_src) (ktr_tgt tt) (ths, im_src, im_tgt, st_src, st, r_shared))
+        (LSIM: r f_src true r_ctx (o, itr_src) (ktr_tgt tt) (ths, im_src, im_tgt, st_src, st, r_shared))
       :
-      lsim_indC tid r RR f_src f_tgt r_ctx (o, itr_src) (trigger (Put st) >>= ktr_tgt) (ths, im_src, im_tgt, st_src, st_tgt, r_shared)
+      lsim_indC tid RR r f_src f_tgt r_ctx (o, itr_src) (trigger (Put st) >>= ktr_tgt) (ths, im_src, im_tgt, st_src, st_tgt, r_shared)
     | lsim_indC_getR
         f_src f_tgt r_ctx o
         ths im_src im_tgt st_src st_tgt r_shared
         itr_src ktr_tgt
-        (LSIM: r _ _ RR f_src true r_ctx (o, itr_src) (ktr_tgt st_tgt) (ths, im_src, im_tgt, st_src, st_tgt, r_shared))
+        (LSIM: r f_src true r_ctx (o, itr_src) (ktr_tgt st_tgt) (ths, im_src, im_tgt, st_src, st_tgt, r_shared))
       :
-      lsim_indC tid r RR f_src f_tgt r_ctx (o, itr_src) (trigger (@Get _) >>= ktr_tgt) (ths, im_src, im_tgt, st_src, st_tgt, r_shared)
+      lsim_indC tid RR r f_src f_tgt r_ctx (o, itr_src) (trigger (@Get _) >>= ktr_tgt) (ths, im_src, im_tgt, st_src, st_tgt, r_shared)
     | lsim_indC_tidR
         f_src f_tgt r_ctx o
         ths im_src im_tgt st_src st_tgt r_shared
         itr_src ktr_tgt
-        (LSIM: r _ _ RR f_src true r_ctx (o, itr_src) (ktr_tgt tid) (ths, im_src, im_tgt, st_src, st_tgt, r_shared))
+        (LSIM: r f_src true r_ctx (o, itr_src) (ktr_tgt tid) (ths, im_src, im_tgt, st_src, st_tgt, r_shared))
       :
-      lsim_indC tid r RR f_src f_tgt r_ctx (o, itr_src) (trigger (GetTid) >>= ktr_tgt) (ths, im_src, im_tgt, st_src, st_tgt, r_shared)
+      lsim_indC tid RR r f_src f_tgt r_ctx (o, itr_src) (trigger (GetTid) >>= ktr_tgt) (ths, im_src, im_tgt, st_src, st_tgt, r_shared)
     | lsim_indC_fairR
         f_src f_tgt r_ctx o
         ths im_src im_tgt0 st_src st_tgt r_shared
         f itr_src ktr_tgt
         (LSIM: forall im_tgt1
                  (FAIR: fair_update im_tgt0 im_tgt1 (sum_fmap_r f)),
-            (<<LSIM: r _ _ RR f_src true r_ctx (o, itr_src) (ktr_tgt tt) (ths, im_src, im_tgt1, st_src, st_tgt, r_shared)>>))
+            (<<LSIM: r f_src true r_ctx (o, itr_src) (ktr_tgt tt) (ths, im_src, im_tgt1, st_src, st_tgt, r_shared)>>))
       :
-      lsim_indC tid r RR f_src f_tgt r_ctx (o, itr_src) (trigger (Fair f) >>= ktr_tgt) (ths, im_src, im_tgt0, st_src, st_tgt, r_shared)
+      lsim_indC tid RR r f_src f_tgt r_ctx (o, itr_src) (trigger (Fair f) >>= ktr_tgt) (ths, im_src, im_tgt0, st_src, st_tgt, r_shared)
 
     | lsim_indC_observe
         f_src f_tgt r_ctx o
         ths im_src im_tgt st_src st_tgt r_shared
         fn args ktr_src ktr_tgt
         (LSIM: forall ret,
-            r _ _ RR true true r_ctx (o, ktr_src ret) (ktr_tgt ret) (ths, im_src, im_tgt, st_src, st_tgt, r_shared))
+            r true true r_ctx (o, ktr_src ret) (ktr_tgt ret) (ths, im_src, im_tgt, st_src, st_tgt, r_shared))
       :
-      lsim_indC tid r RR f_src f_tgt r_ctx (o, trigger (Observe fn args) >>= ktr_src) (trigger (Observe fn args) >>= ktr_tgt) (ths, im_src, im_tgt, st_src, st_tgt, r_shared)
+      lsim_indC tid RR r f_src f_tgt r_ctx (o, trigger (Observe fn args) >>= ktr_src) (trigger (Observe fn args) >>= ktr_tgt) (ths, im_src, im_tgt, st_src, st_tgt, r_shared)
 
     | lsim_indC_yieldR
         f_src f_tgt r_ctx0 o0
@@ -355,30 +354,30 @@ Section PRIMIVIESIM.
                  im_tgt2
                  (TGT: fair_update im_tgt1 im_tgt2 (sum_fmap_l (tids_fmap tid ths1))),
           exists o1,
-            (<<LSIM: r _ _ RR true true r_ctx1 (o1, trigger (Yield) >>= ktr_src) (ktr_tgt tt) (ths1, im_src1, im_tgt2, st_src1, st_tgt1, r_shared1)>>) /\
+            (<<LSIM: r true true r_ctx1 (o1, trigger (Yield) >>= ktr_src) (ktr_tgt tt) (ths1, im_src1, im_tgt2, st_src1, st_tgt1, r_shared1)>>) /\
               (<<STUTTER: (wf_stt R_src R_tgt).(lt) o1 o0>>))
       :
-      lsim_indC tid r RR f_src f_tgt r_ctx0 (o0, trigger (Yield) >>= ktr_src) (trigger (Yield) >>= ktr_tgt) (ths0, im_src0, im_tgt0, st_src0, st_tgt0, r_shared0)
+      lsim_indC tid RR r f_src f_tgt r_ctx0 (o0, trigger (Yield) >>= ktr_src) (trigger (Yield) >>= ktr_tgt) (ths0, im_src0, im_tgt0, st_src0, st_tgt0, r_shared0)
     | lsim_indC_yieldL
         f_src f_tgt r_ctx o0
         ths im_src0 im_tgt st_src st_tgt r_shared
         ktr_src itr_tgt
         (LSIM: exists im_src1 o1,
             (<<FAIR: fair_update im_src0 im_src1 (sum_fmap_l (tids_fmap tid ths))>>) /\
-              (<<LSIM: r _ _ RR true f_tgt r_ctx (o1, ktr_src tt) itr_tgt (ths, im_src1, im_tgt, st_src, st_tgt, r_shared)>>))
+              (<<LSIM: r true f_tgt r_ctx (o1, ktr_src tt) itr_tgt (ths, im_src1, im_tgt, st_src, st_tgt, r_shared)>>))
       :
-      lsim_indC tid r RR f_src f_tgt r_ctx (o0, trigger (Yield) >>= ktr_src) itr_tgt (ths, im_src0, im_tgt, st_src, st_tgt, r_shared)
+      lsim_indC tid RR r f_src f_tgt r_ctx (o0, trigger (Yield) >>= ktr_src) itr_tgt (ths, im_src0, im_tgt, st_src, st_tgt, r_shared)
 
     | lsim_indC_progress
         r_ctx o
         ths im_src im_tgt st_src st_tgt r_shared
         itr_src itr_tgt
-        (LSIM: r _ _ RR false false r_ctx (o, itr_src) itr_tgt (ths, im_src, im_tgt, st_src, st_tgt, r_shared))
+        (LSIM: r false false r_ctx (o, itr_src) itr_tgt (ths, im_src, im_tgt, st_src, st_tgt, r_shared))
       :
-      lsim_indC tid r RR true true r_ctx (o, itr_src) itr_tgt (ths, im_src, im_tgt, st_src, st_tgt, r_shared)
+      lsim_indC tid RR r true true r_ctx (o, itr_src) itr_tgt (ths, im_src, im_tgt, st_src, st_tgt, r_shared)
   .
 
-  Lemma lsim_indC_mon tid: monotone9 (lsim_indC tid).
+  Lemma lsim_indC_mon tid R0 R1 (RR: R0 -> R1 -> _ -> _): monotone6 (lsim_indC tid RR).
   Proof.
     ii. inv IN; try (econs; eauto; fail).
     { des; econs; eauto. }
@@ -390,184 +389,184 @@ Section PRIMIVIESIM.
 
   Hint Resolve lsim_indC_mon: paco.
 
-  Lemma lsim_indC_wrepectful tid: wrespectful9 (fun r => pind9 (__lsim tid r) top9) (lsim_indC tid).
+  Lemma lsim_indC_wrepectful tid R0 R1 (RR: R0 -> R1 -> _ -> _):
+    wrespectful6 (fun r => pind6 (__lsim tid RR r) top6) (lsim_indC tid RR).
   Proof.
     econs; eauto with paco.
-    i. eapply pind9_fold. inv PR.
+    i. eapply pind6_fold. inv PR.
     { econs 1; eauto. }
     { econs 2; eauto. split; ss.
-      eapply GF in LSIM. eapply pind9_mon_gen; ss. eauto.
-      i. eapply __lsim_mon. 2: eauto. i. eapply rclo9_base; auto.
+      eapply GF in LSIM. eapply pind6_mon_gen; ss. eauto.
+      i. eapply __lsim_mon. 2: eauto. i. eapply rclo6_base; auto.
     }
     { des. econs 3; eauto. esplits; eauto. split; ss.
-      eapply GF in LSIM. eapply pind9_mon_gen; ss. eauto.
-      i. eapply __lsim_mon. 2: eauto. i. eapply rclo9_base; auto.
+      eapply GF in LSIM. eapply pind6_mon_gen; ss. eauto.
+      i. eapply __lsim_mon. 2: eauto. i. eapply rclo6_base; auto.
     }
     { econs 4; eauto. split; ss.
-      eapply GF in LSIM. eapply pind9_mon_gen; ss. eauto.
-      i. eapply __lsim_mon. 2: eauto. i. eapply rclo9_base; auto.
+      eapply GF in LSIM. eapply pind6_mon_gen; ss. eauto.
+      i. eapply __lsim_mon. 2: eauto. i. eapply rclo6_base; auto.
     }
     { econs 5; eauto. split; ss.
-      eapply GF in LSIM. eapply pind9_mon_gen; ss. eauto.
-      i. eapply __lsim_mon. 2: eauto. i. eapply rclo9_base; auto.
+      eapply GF in LSIM. eapply pind6_mon_gen; ss. eauto.
+      i. eapply __lsim_mon. 2: eauto. i. eapply rclo6_base; auto.
     }
     { econs 6; eauto. split; ss.
-      eapply GF in LSIM. eapply pind9_mon_gen; ss. eauto.
-      i. eapply __lsim_mon. 2: eauto. i. eapply rclo9_base; auto.
+      eapply GF in LSIM. eapply pind6_mon_gen; ss. eauto.
+      i. eapply __lsim_mon. 2: eauto. i. eapply rclo6_base; auto.
     }
     { econs 7; eauto. }
     { des. econs 8; eauto. esplits; eauto. split; ss.
-      eapply GF in LSIM0. eapply pind9_mon_gen; ss. eauto.
-      i. eapply __lsim_mon. 2: eauto. i. eapply rclo9_base; auto.
+      eapply GF in LSIM0. eapply pind6_mon_gen; ss. eauto.
+      i. eapply __lsim_mon. 2: eauto. i. eapply rclo6_base; auto.
     }
     { econs 9; eauto. split; ss.
-      eapply GF in LSIM. eapply pind9_mon_gen; ss. eauto.
-      i. eapply __lsim_mon. 2: eauto. i. eapply rclo9_base; auto.
+      eapply GF in LSIM. eapply pind6_mon_gen; ss. eauto.
+      i. eapply __lsim_mon. 2: eauto. i. eapply rclo6_base; auto.
     }
     { econs 10; eauto. i. specialize (LSIM x). split; ss.
-      eapply GF in LSIM. eapply pind9_mon_gen; ss. eauto.
-      i. eapply __lsim_mon. 2: eauto. i. eapply rclo9_base; auto.
+      eapply GF in LSIM. eapply pind6_mon_gen; ss. eauto.
+      i. eapply __lsim_mon. 2: eauto. i. eapply rclo6_base; auto.
     }
     { econs 11; eauto. split; ss.
-      eapply GF in LSIM. eapply pind9_mon_gen; ss. eauto.
-      i. eapply __lsim_mon. 2: eauto. i. eapply rclo9_base; auto.
+      eapply GF in LSIM. eapply pind6_mon_gen; ss. eauto.
+      i. eapply __lsim_mon. 2: eauto. i. eapply rclo6_base; auto.
     }
     { econs 12; eauto. split; ss.
-      eapply GF in LSIM. eapply pind9_mon_gen; ss. eauto.
-      i. eapply __lsim_mon. 2: eauto. i. eapply rclo9_base; auto.
+      eapply GF in LSIM. eapply pind6_mon_gen; ss. eauto.
+      i. eapply __lsim_mon. 2: eauto. i. eapply rclo6_base; auto.
     }
     { econs 13; eauto. split; ss.
-      eapply GF in LSIM. eapply pind9_mon_gen; ss. eauto.
-      i. eapply __lsim_mon. 2: eauto. i. eapply rclo9_base; auto.
+      eapply GF in LSIM. eapply pind6_mon_gen; ss. eauto.
+      i. eapply __lsim_mon. 2: eauto. i. eapply rclo6_base; auto.
     }
     { econs 14; eauto. i. specialize (LSIM _ FAIR). split; ss.
-      eapply GF in LSIM. eapply pind9_mon_gen; ss. eauto.
-      i. eapply __lsim_mon. 2: eauto. i. eapply rclo9_base; auto.
+      eapply GF in LSIM. eapply pind6_mon_gen; ss. eauto.
+      i. eapply __lsim_mon. 2: eauto. i. eapply rclo6_base; auto.
     }
     { econs 15; eauto. i. specialize (LSIM ret).
-      eapply rclo9_base; auto.
+      eapply rclo6_base; auto.
     }
     { econs 16; eauto. i. specialize (LSIM _ _ _ _ _ _ _ INV0 VALID0 _ TGT).
       des. esplits; eauto.
-      eapply rclo9_base; auto.
+      eapply rclo6_base; auto.
     }
     { des. econs 17; eauto. esplits; eauto. split; ss.
-      eapply GF in LSIM0. eapply pind9_mon_gen; ss. eauto.
-      i. eapply __lsim_mon. 2: eauto. i. eapply rclo9_base; auto.
+      eapply GF in LSIM0. eapply pind6_mon_gen; ss. eauto.
+      i. eapply __lsim_mon. 2: eauto. i. eapply rclo6_base; auto.
     }
-    { econs 18; eauto. eapply rclo9_base; auto. }
+    { econs 18; eauto. eapply rclo6_base; auto. }
   Qed.
 
-  Lemma lsim_indC_spec tid:
-    (lsim_indC tid) <10= gupaco9 (fun r => pind9 (__lsim tid r) top9) (cpn9 (fun r => pind9 (__lsim tid r) top9)).
+  Lemma lsim_indC_spec tid R0 R1 (RR: R0 -> R1 -> _ -> _):
+    (lsim_indC tid RR) <7= gupaco6 (fun r => pind6 (__lsim tid RR r) top6) (cpn6 (fun r => pind6 (__lsim tid RR r) top6)).
   Proof.
-    i. eapply wrespect9_uclo; eauto with paco.
+    i. eapply wrespect6_uclo; eauto with paco.
     { eapply lsim_mon. }
     eapply lsim_indC_wrepectful.
   Qed.
 
 
-  Variant lsim_resetC
-          (r: forall R_src R_tgt (RR: R_src -> R_tgt -> URA.car -> shared_rel), bool -> bool -> URA.car -> ((wf_stt R_src R_tgt).(T) * itree srcE R_src) -> itree tgtE R_tgt -> shared_rel)
-          R_src R_tgt (RR: R_src -> R_tgt -> URA.car -> shared_rel)
+  Variant lsim_resetC R_src R_tgt (RR: R_src -> R_tgt -> URA.car -> shared_rel)
+          (r: bool -> bool -> URA.car -> ((wf_stt R_src R_tgt).(T) * itree srcE R_src) -> itree tgtE R_tgt -> shared_rel)
     :
     bool -> bool -> URA.car -> ((wf_stt R_src R_tgt).(T) * itree srcE R_src) -> itree tgtE R_tgt -> shared_rel :=
     | lsim_resetC_intro
         src tgt shr r_ctx
         ps0 pt0 ps1 pt1
-        (REL: r _ _ RR ps1 pt1 r_ctx src tgt shr)
+        (REL: r ps1 pt1 r_ctx src tgt shr)
         (SRC: ps1 = true -> ps0 = true)
         (TGT: pt1 = true -> pt0 = true)
       :
-      lsim_resetC r RR ps0 pt0 r_ctx src tgt shr
+      lsim_resetC RR r ps0 pt0 r_ctx src tgt shr
   .
 
-  Lemma lsim_resetC_spec tid
+  Lemma lsim_resetC_spec tid R_src R_tgt (RR: R_src -> R_tgt -> URA.car -> shared_rel)
     :
-    lsim_resetC <10= gupaco9 (fun r => pind9 (__lsim tid r) top9) (cpn9 (fun r => pind9 (__lsim tid r) top9)).
+    lsim_resetC RR <7= gupaco6 (fun r => pind6 (__lsim tid RR r) top6) (cpn6 (fun r => pind6 (__lsim tid RR r) top6)).
   Proof.
-    eapply wrespect9_uclo; eauto with paco.
+    eapply wrespect6_uclo; eauto with paco.
     { eapply lsim_mon. }
     econs.
     { ii. inv IN. econs; eauto. }
     i. inv PR. eapply GF in REL.
-    eapply pind9_acc in REL.
-    instantiate (1:= (fun R0 R1 (RR: R0 -> R1 -> URA.car -> shared_rel) ps1 pt1 r_ctx src tgt shr =>
+    eapply pind6_acc in REL.
+    instantiate (1:= (fun ps1 pt1 r_ctx src tgt shr =>
                         forall ps0 pt0,
                           (ps1 = true -> ps0 = true) ->
                           (pt1 = true -> pt0 = true) ->
-                          pind9 (__lsim tid (rclo9 lsim_resetC r)) top9 R0 R1 RR ps0 pt0 r_ctx src tgt shr)) in REL; eauto.
-    ss. i. eapply pind9_unfold in PR.
+                          pind6 (__lsim tid RR (rclo6 (lsim_resetC RR) r)) top6 ps0 pt0 r_ctx src tgt shr)) in REL; eauto.
+    ss. i. eapply pind6_unfold in PR.
     2:{ eapply _lsim_mon. }
     rename PR into LSIM. inv LSIM.
 
-    { eapply pind9_fold. econs; eauto. }
+    { eapply pind6_fold. econs; eauto. }
 
     { destruct LSIM0 as [LSIM0 IND]. clear LSIM0.
-      eapply pind9_fold. eapply lsim_tauL. split; ss.
+      eapply pind6_fold. eapply lsim_tauL. split; ss.
       hexploit IH; eauto.
     }
 
-    { des. eapply pind9_fold. eapply lsim_chooseL. esplits; eauto. split; ss.
+    { des. eapply pind6_fold. eapply lsim_chooseL. esplits; eauto. split; ss.
       destruct LSIM0 as [LSIM0 IND]. hexploit IH; eauto.
     }
 
-    { eapply pind9_fold. eapply lsim_putL. split; ss.
+    { eapply pind6_fold. eapply lsim_putL. split; ss.
       destruct LSIM0 as [LSIM0 IND]. hexploit IH; eauto.
     }
 
-    { eapply pind9_fold. eapply lsim_getL. split; ss.
+    { eapply pind6_fold. eapply lsim_getL. split; ss.
       destruct LSIM0 as [LSIM0 IND]. hexploit IH; eauto.
     }
 
-    { eapply pind9_fold. eapply lsim_tidL. split; ss.
+    { eapply pind6_fold. eapply lsim_tidL. split; ss.
       destruct LSIM0 as [LSIM0 IND]. hexploit IH; eauto.
     }
 
-    { eapply pind9_fold. eapply lsim_UB. }
+    { eapply pind6_fold. eapply lsim_UB. }
 
-    { des. eapply pind9_fold. eapply lsim_fairL. esplits; eauto. split; ss.
+    { des. eapply pind6_fold. eapply lsim_fairL. esplits; eauto. split; ss.
       destruct LSIM as [LSIM IND]. hexploit IH; eauto.
     }
 
     { destruct LSIM0 as [LSIM0 IND]. clear LSIM0.
-      eapply pind9_fold. eapply lsim_tauR. split; ss.
+      eapply pind6_fold. eapply lsim_tauR. split; ss.
       hexploit IH. eauto. all: eauto.
     }
 
-    { eapply pind9_fold. eapply lsim_chooseR. i. split; ss. specialize (LSIM0 x).
+    { eapply pind6_fold. eapply lsim_chooseR. i. split; ss. specialize (LSIM0 x).
       destruct LSIM0 as [LSIM0 IND]. hexploit IH; eauto.
     }
 
-    { eapply pind9_fold. eapply lsim_putR. split; ss.
+    { eapply pind6_fold. eapply lsim_putR. split; ss.
       destruct LSIM0 as [LSIM0 IND]. hexploit IH; eauto.
     }
 
-    { eapply pind9_fold. eapply lsim_getR. split; ss.
+    { eapply pind6_fold. eapply lsim_getR. split; ss.
       destruct LSIM0 as [LSIM0 IND]. hexploit IH; eauto.
     }
 
-    { eapply pind9_fold. eapply lsim_tidR. split; ss.
+    { eapply pind6_fold. eapply lsim_tidR. split; ss.
       destruct LSIM0 as [LSIM0 IND]. hexploit IH; eauto.
     }
 
-    { eapply pind9_fold. eapply lsim_fairR. i. split; ss. specialize (LSIM0 _ FAIR).
+    { eapply pind6_fold. eapply lsim_fairR. i. split; ss. specialize (LSIM0 _ FAIR).
       des. destruct LSIM0 as [LSIM0 IND]. hexploit IH; eauto.
     }
 
-    { eapply pind9_fold. eapply lsim_observe. i. eapply rclo9_base. auto. }
+    { eapply pind6_fold. eapply lsim_observe. i. eapply rclo6_base. auto. }
 
-    { eapply pind9_fold. eapply lsim_yieldR; eauto. i.
+    { eapply pind6_fold. eapply lsim_yieldR; eauto. i.
       hexploit LSIM0; eauto. clear LSIM0. intros LSIM0. des. esplits; eauto.
-      eapply rclo9_base. auto.
+      eapply rclo6_base. auto.
     }
 
-    { des. eapply pind9_fold. eapply lsim_yieldL. esplits; eauto. split; ss.
+    { des. eapply pind6_fold. eapply lsim_yieldL. esplits; eauto. split; ss.
       destruct LSIM as [LSIM IND]. hexploit IH; eauto.
     }
 
     { hexploit H; ss; i. hexploit H0; ss; i. clarify.
-      eapply pind9_fold. eapply lsim_progress. eapply rclo9_base; auto. }
+      eapply pind6_fold. eapply lsim_progress. eapply rclo6_base; auto. }
   Qed.
 
   Lemma lsim_reset_prog
@@ -583,7 +582,7 @@ Section PRIMIVIESIM.
   Proof.
     ginit.
     { eapply lsim_mon. }
-    { eapply cpn9_wcompat. eapply lsim_mon. }
+    { eapply cpn6_wcompat. eapply lsim_mon. }
     guclo lsim_resetC_spec.
     { eapply lsim_mon. }
     econs; eauto. gfinal.
@@ -599,193 +598,190 @@ Section PRIMIVIESIM.
     :
     forall ps pt, lsim tid RR ps pt r_ctx src tgt shr.
   Proof.
-    i. revert_until tid. pcofix CIH. i.
+    i. revert_until RR. pcofix CIH. i.
     remember true as ps0 in LSIM at 1. remember true as pt0 in LSIM at 1.
     move LSIM before CIH. revert_until LSIM. punfold LSIM.
     2:{ eapply lsim_mon. }
-    eapply pind9_acc in LSIM.
+    eapply pind6_acc in LSIM.
 
-    { instantiate (1:= (fun R0 R1 (RR: R0 -> R1 -> URA.car -> shared_rel) ps0 pt0 r_ctx src tgt shr =>
+    { instantiate (1:= (fun ps0 pt0 r_ctx src tgt shr =>
                           ps0 = true ->
                           pt0 = true ->
                           forall ps pt,
-                            paco9
-                              (fun r0 =>
-                                 pind9 (__lsim tid r0) top9) r R0 R1 RR ps pt r_ctx src tgt shr)) in LSIM; auto. }
+                            paco6 (fun r0 => pind6 (__lsim tid RR r0) top6) r ps pt r_ctx src tgt shr)) in LSIM; auto. }
 
     ss. clear ps0 pt0 r_ctx src tgt shr LSIM.
-    intros rr DEC IH R0' R1' RR' gps gpt r_ctx src tgt shr LSIM. clear DEC.
+    intros rr DEC IH gps gpt r_ctx src tgt shr LSIM. clear DEC.
     intros Egps Egpt ps pt.
-    eapply pind9_unfold in LSIM.
+    eapply pind6_unfold in LSIM.
     2:{ eapply _lsim_mon. }
     inv LSIM.
 
-    { pfold. eapply pind9_fold. econs; eauto. }
+    { pfold. eapply pind6_fold. econs; eauto. }
 
     { destruct LSIM0 as [LSIM0 IND]. clear LSIM0.
-      pfold. eapply pind9_fold. eapply lsim_tauL. split; ss.
+      pfold. eapply pind6_fold. eapply lsim_tauL. split; ss.
       hexploit IH. eauto. all: eauto. i. punfold H. eapply lsim_mon.
     }
 
-    { des. pfold. eapply pind9_fold. eapply lsim_chooseL. esplits; eauto. split; ss.
+    { des. pfold. eapply pind6_fold. eapply lsim_chooseL. esplits; eauto. split; ss.
       destruct LSIM0 as [LSIM0 IND]. hexploit IH; eauto. i. punfold H. eapply lsim_mon.
     }
 
-    { pfold. eapply pind9_fold. eapply lsim_putL. split; ss.
+    { pfold. eapply pind6_fold. eapply lsim_putL. split; ss.
       destruct LSIM0 as [LSIM0 IND]. hexploit IH; eauto. i. punfold H. eapply lsim_mon.
     }
 
-    { pfold. eapply pind9_fold. eapply lsim_getL. split; ss.
+    { pfold. eapply pind6_fold. eapply lsim_getL. split; ss.
       destruct LSIM0 as [LSIM0 IND]. hexploit IH; eauto. i. punfold H. eapply lsim_mon.
     }
 
-    { pfold. eapply pind9_fold. eapply lsim_tidL. split; ss.
+    { pfold. eapply pind6_fold. eapply lsim_tidL. split; ss.
       destruct LSIM0 as [LSIM0 IND]. hexploit IH; eauto. i. punfold H. eapply lsim_mon.
     }
 
-    { pfold. eapply pind9_fold. eapply lsim_UB. }
+    { pfold. eapply pind6_fold. eapply lsim_UB. }
 
-    { des. pfold. eapply pind9_fold. eapply lsim_fairL. esplits; eauto. split; ss.
+    { des. pfold. eapply pind6_fold. eapply lsim_fairL. esplits; eauto. split; ss.
       destruct LSIM as [LSIM IND]. hexploit IH; eauto. i. punfold H. eapply lsim_mon.
     }
 
     { destruct LSIM0 as [LSIM0 IND]. clear LSIM0.
-      pfold. eapply pind9_fold. eapply lsim_tauR. split; ss.
+      pfold. eapply pind6_fold. eapply lsim_tauR. split; ss.
       hexploit IH. eauto. all: eauto. i. punfold H. eapply lsim_mon.
     }
 
-    { pfold. eapply pind9_fold. eapply lsim_chooseR. i. split; ss. specialize (LSIM0 x).
+    { pfold. eapply pind6_fold. eapply lsim_chooseR. i. split; ss. specialize (LSIM0 x).
       destruct LSIM0 as [LSIM0 IND]. hexploit IH; eauto. i. punfold H. eapply lsim_mon.
     }
 
-    { pfold. eapply pind9_fold. eapply lsim_putR. split; ss.
+    { pfold. eapply pind6_fold. eapply lsim_putR. split; ss.
       destruct LSIM0 as [LSIM0 IND]. hexploit IH; eauto. i. punfold H. eapply lsim_mon.
     }
 
-    { pfold. eapply pind9_fold. eapply lsim_getR. split; ss.
+    { pfold. eapply pind6_fold. eapply lsim_getR. split; ss.
       destruct LSIM0 as [LSIM0 IND]. hexploit IH; eauto. i. punfold H. eapply lsim_mon.
     }
 
-    { pfold. eapply pind9_fold. eapply lsim_tidR. split; ss.
+    { pfold. eapply pind6_fold. eapply lsim_tidR. split; ss.
       destruct LSIM0 as [LSIM0 IND]. hexploit IH; eauto. i. punfold H. eapply lsim_mon.
     }
 
-    { pfold. eapply pind9_fold. eapply lsim_fairR. i. split; ss. specialize (LSIM0 _ FAIR).
+    { pfold. eapply pind6_fold. eapply lsim_fairR. i. split; ss. specialize (LSIM0 _ FAIR).
       des. destruct LSIM0 as [LSIM0 IND]. hexploit IH; eauto. i. punfold H. eapply lsim_mon.
     }
 
-    { pfold. eapply pind9_fold. eapply lsim_observe. i. eapply upaco9_mon_bot; eauto. }
+    { pfold. eapply pind6_fold. eapply lsim_observe. i. eapply upaco6_mon_bot; eauto. }
 
-    { pfold. eapply pind9_fold. eapply lsim_yieldR; eauto. i.
+    { pfold. eapply pind6_fold. eapply lsim_yieldR; eauto. i.
       hexploit LSIM0; eauto. clear LSIM0. intros LSIM0. des. esplits; eauto.
-      eapply upaco9_mon_bot; eauto.
+      eapply upaco6_mon_bot; eauto.
     }
 
-    { des. pfold. eapply pind9_fold. eapply lsim_yieldL. esplits; eauto. split; ss.
+    { des. pfold. eapply pind6_fold. eapply lsim_yieldL. esplits; eauto. split; ss.
       destruct LSIM as [LSIM IND]. hexploit IH; eauto. i. punfold H. eapply lsim_mon.
     }
 
-    { pclearbot. eapply paco9_mon_bot. eapply lsim_reset_prog. eauto. all: ss. }
+    { pclearbot. eapply paco6_mon_bot. eapply lsim_reset_prog. eauto. all: ss. }
 
   Qed.
 
 
-  Variant lsim_ord_weakC
-          (r: forall R_src R_tgt (RR: R_src -> R_tgt -> URA.car -> shared_rel), bool -> bool -> URA.car -> ((wf_stt R_src R_tgt).(T) * itree srcE R_src) -> itree tgtE R_tgt -> shared_rel)
-          R_src R_tgt (RR: R_src -> R_tgt -> URA.car -> shared_rel)
+  Variant lsim_ord_weakC R_src R_tgt (RR: R_src -> R_tgt -> URA.car -> shared_rel)
+          (r: bool -> bool -> URA.car -> ((wf_stt R_src R_tgt).(T) * itree srcE R_src) -> itree tgtE R_tgt -> shared_rel)
     :
     bool -> bool -> URA.car -> ((wf_stt R_src R_tgt).(T) * itree srcE R_src) -> itree tgtE R_tgt -> shared_rel :=
     | lsim_ord_weakC_intro
         src tgt shr r_ctx ps pt o0 o1
-        (REL: r _ _ RR ps pt r_ctx (o0, src) tgt shr)
+        (REL: r ps pt r_ctx (o0, src) tgt shr)
         (LE: (wf_stt R_src R_tgt).(le) o0 o1)
       :
-      lsim_ord_weakC r RR ps pt r_ctx (o1, src) tgt shr
+      lsim_ord_weakC RR r ps pt r_ctx (o1, src) tgt shr
   .
 
-  Lemma lsim_ord_weakC_spec tid
+  Lemma lsim_ord_weakC_spec tid R_src R_tgt (RR: R_src -> R_tgt -> URA.car -> shared_rel)
     :
-    lsim_ord_weakC <10= gupaco9 (fun r => pind9 (__lsim tid r) top9) (cpn9 (fun r => pind9 (__lsim tid r) top9)).
+    lsim_ord_weakC RR <7= gupaco6 (fun r => pind6 (__lsim tid RR r) top6) (cpn6 (fun r => pind6 (__lsim tid RR r) top6)).
   Proof.
-    eapply wrespect9_uclo; eauto with paco.
+    eapply wrespect6_uclo; eauto with paco.
     { eapply lsim_mon. }
     econs.
     { ii. inv IN. econs; eauto. }
     i. inv PR. destruct LE0 as [EQ | LT].
-    { clarify. eapply pind9_mon_gen. eapply GF; eauto. 2: ss.
-      i. eapply __lsim_mon. 2: eauto. i. eapply rclo9_base. auto.
+    { clarify. eapply pind6_mon_gen. eapply GF; eauto. 2: ss.
+      i. eapply __lsim_mon. 2: eauto. i. eapply rclo6_base. auto.
     }
     eapply GF in REL.
     remember (o0, src) as osrc. rename REL into LSIM.
     move LSIM before GF. revert_until LSIM.
-    pattern x0, x1, x2, x3, x4, x5, osrc, x7, x8.
-    revert x0 x1 x2 x3 x4 x5 osrc x7 x8 LSIM. apply pind9_acc.
-    intros rr DEC IH. clear DEC. intros R0 R1 LRR ps pt r_ctx osrc tgt shr LSIM.
+    pattern x0, x1, x2, osrc, x4, x5.
+    revert x0 x1 x2 osrc x4 x5 LSIM. apply pind6_acc.
+    intros rr DEC IH. clear DEC. intros ps pt r_ctx osrc tgt shr LSIM.
     i; clarify.
-    eapply pind9_unfold in LSIM.
+    eapply pind6_unfold in LSIM.
     2:{ eapply _lsim_mon. }
     inv LSIM.
 
-    { eapply pind9_fold. econs 1; eauto. }
-    { eapply pind9_fold. econs 2; eauto.
+    { eapply pind6_fold. econs 1; eauto. }
+    { eapply pind6_fold. econs 2; eauto.
       split; ss. destruct LSIM0 as [LSIM IND]. eapply IH in IND; eauto.
     }
-    { eapply pind9_fold. econs 3; eauto.
+    { eapply pind6_fold. econs 3; eauto.
       des. exists x.
       split; ss. destruct LSIM0 as [LSIM IND]. eapply IH in IND; eauto.
     }
-    { eapply pind9_fold. econs 4; eauto.
+    { eapply pind6_fold. econs 4; eauto.
       split; ss. destruct LSIM0 as [LSIM IND]. eapply IH in IND; eauto.
     }
-    { eapply pind9_fold. econs 5; eauto.
+    { eapply pind6_fold. econs 5; eauto.
       split; ss. destruct LSIM0 as [LSIM IND]. eapply IH in IND; eauto.
     }
-    { eapply pind9_fold. econs 6; eauto.
+    { eapply pind6_fold. econs 6; eauto.
       split; ss. destruct LSIM0 as [LSIM IND]. eapply IH in IND; eauto.
     }
-    { eapply pind9_fold. econs 7; eauto. }
-    { eapply pind9_fold. econs 8; eauto.
+    { eapply pind6_fold. econs 7; eauto. }
+    { eapply pind6_fold. econs 8; eauto.
       des. esplits; eauto.
       split; ss. destruct LSIM as [LSIM IND]. eapply IH in IND; eauto.
     }
-    { eapply pind9_fold. econs 9; eauto.
+    { eapply pind6_fold. econs 9; eauto.
       split; ss. destruct LSIM0 as [LSIM IND]. eapply IH in IND; eauto.
     }
-    { eapply pind9_fold. econs 10; eauto.
+    { eapply pind6_fold. econs 10; eauto.
       i. specialize (LSIM0 x).
       split; ss. destruct LSIM0 as [LSIM IND]. eapply IH in IND; eauto.
     }
-    { eapply pind9_fold. econs 11; eauto.
+    { eapply pind6_fold. econs 11; eauto.
       split; ss. destruct LSIM0 as [LSIM IND]. eapply IH in IND; eauto.
     }
-    { eapply pind9_fold. econs 12; eauto.
+    { eapply pind6_fold. econs 12; eauto.
       split; ss. destruct LSIM0 as [LSIM IND]. eapply IH in IND; eauto.
     }
-    { eapply pind9_fold. econs 13; eauto.
+    { eapply pind6_fold. econs 13; eauto.
       split; ss. destruct LSIM0 as [LSIM IND]. eapply IH in IND; eauto.
     }
-    { eapply pind9_fold. econs 14; eauto.
+    { eapply pind6_fold. econs 14; eauto.
       i. specialize (LSIM0 _ FAIR).
       split; ss. destruct LSIM0 as [LSIM IND]. eapply IH in IND; eauto.
     }
-    { eapply pind9_fold. econs 15; eauto.
+    { eapply pind6_fold. econs 15; eauto.
       i. specialize (LSIM0 ret).
-      eapply rclo9_clo_base. econs; eauto. right. auto.
+      eapply rclo6_clo_base. econs; eauto. right. auto.
     }
 
-    { eapply pind9_fold. eapply lsim_yieldR; eauto.
+    { eapply pind6_fold. eapply lsim_yieldR; eauto.
       i. hexploit LSIM0; clear LSIM0; eauto; intro LSIM. des. esplits; eauto.
-      eapply rclo9_clo_base. econs; eauto. right. auto.
+      eapply rclo6_clo_base. econs; eauto. right. auto.
     }
 
-    { eapply pind9_fold. eapply lsim_yieldL; eauto.
+    { eapply pind6_fold. eapply lsim_yieldL; eauto.
       des. esplits; eauto. destruct LSIM as [LSIM IND].
-      split; ss. eapply pind9_mon_gen. eapply LSIM. 2: ss.
-      i. eapply __lsim_mon. 2: eapply PR. i. eapply rclo9_base; eauto.
+      split; ss. eapply pind6_mon_gen. eapply LSIM. 2: ss.
+      i. eapply __lsim_mon. 2: eapply PR. i. eapply rclo6_base; eauto.
     }
 
-    { eapply pind9_fold. eapply lsim_progress.
-      eapply rclo9_clo_base. econs; eauto. right. auto.
+    { eapply pind6_fold. eapply lsim_progress.
+      eapply rclo6_clo_base. econs; eauto. right. auto.
     }
 
   Qed.
@@ -801,7 +797,7 @@ Section PRIMIVIESIM.
   Proof.
     ginit.
     { eapply lsim_mon. }
-    { eapply cpn9_wcompat. eapply lsim_mon. }
+    { eapply cpn6_wcompat. eapply lsim_mon. }
     guclo lsim_ord_weakC_spec.
     { eapply lsim_mon. }
     econs; eauto. gfinal.
