src/NoSync2Stutter.v
@@ -48,9 +48,8 @@ Section GENORDER.
   Let wf_stt {R0 R1} := @ord_tree_WF (A R0 R1).
 
   Variant _geno
-          (tid: thread_id) R_src R_tgt
-          (geno: forall (RR: R_src -> R_tgt -> URA.car -> shared_rel), bool -> bool -> URA.car -> ((@wf_stt R_src R_tgt).(T) * itree srcE R_src) -> itree tgtE R_tgt -> shared_rel)
-          (RR: R_src -> R_tgt -> URA.car -> shared_rel)
+          (tid: thread_id) R_src R_tgt (RR: R_src -> R_tgt -> URA.car -> shared_rel)
+          (geno: bool -> bool -> URA.car -> ((@wf_stt R_src R_tgt).(T) * itree srcE R_src) -> itree tgtE R_tgt -> shared_rel)
     :
     bool -> bool -> URA.car -> ((@wf_stt R_src R_tgt).(T) * itree srcE R_src) -> itree tgtE R_tgt -> shared_rel :=
   | geno_ret
@@ -60,112 +59,112 @@ Section GENORDER.
       (LT: wf_stt.(lt) o0 o)
       (GENO: RR r_src r_tgt r_ctx (ths, im_src, im_tgt, st_src, st_tgt, r_shared))
     :
-    _geno tid geno RR f_src f_tgt r_ctx (o, Ret r_src) (Ret r_tgt) (ths, im_src, im_tgt, st_src, st_tgt, r_shared)
+    _geno tid RR geno f_src f_tgt r_ctx (o, Ret r_src) (Ret r_tgt) (ths, im_src, im_tgt, st_src, st_tgt, r_shared)
 
   | geno_tauL
       f_src f_tgt r_ctx o
       ths im_src im_tgt st_src st_tgt r_shared
       itr_src itr_tgt
-      (GENO: geno RR true f_tgt r_ctx (o, itr_src) itr_tgt (ths, im_src, im_tgt, st_src, st_tgt, r_shared))
+      (GENO: geno true f_tgt r_ctx (o, itr_src) itr_tgt (ths, im_src, im_tgt, st_src, st_tgt, r_shared))
     :
-    _geno tid geno RR f_src f_tgt r_ctx (o, Tau itr_src) itr_tgt (ths, im_src, im_tgt, st_src, st_tgt, r_shared)
+    _geno tid RR geno f_src f_tgt r_ctx (o, Tau itr_src) itr_tgt (ths, im_src, im_tgt, st_src, st_tgt, r_shared)
   | geno_chooseL
       f_src f_tgt r_ctx o
       ths im_src im_tgt st_src st_tgt r_shared
       X ktr_src itr_tgt
-      (GENO: exists x, geno RR true f_tgt r_ctx (o, ktr_src x) itr_tgt (ths, im_src, im_tgt, st_src, st_tgt, r_shared))
+      (GENO: exists x, geno true f_tgt r_ctx (o, ktr_src x) itr_tgt (ths, im_src, im_tgt, st_src, st_tgt, r_shared))
     :
-    _geno tid geno RR f_src f_tgt r_ctx (o, trigger (Choose X) >>= ktr_src) itr_tgt (ths, im_src, im_tgt, st_src, st_tgt, r_shared)
+    _geno tid RR geno f_src f_tgt r_ctx (o, trigger (Choose X) >>= ktr_src) itr_tgt (ths, im_src, im_tgt, st_src, st_tgt, r_shared)
   | geno_putL
       f_src f_tgt r_ctx o
       ths im_src im_tgt st_src st_tgt r_shared
       st ktr_src itr_tgt
-      (GENO: geno RR true f_tgt r_ctx (o, ktr_src tt) itr_tgt (ths, im_src, im_tgt, st, st_tgt, r_shared))
+      (GENO: geno true f_tgt r_ctx (o, ktr_src tt) itr_tgt (ths, im_src, im_tgt, st, st_tgt, r_shared))
     :
-    _geno tid geno RR f_src f_tgt r_ctx (o, trigger (Put st) >>= ktr_src) itr_tgt (ths, im_src, im_tgt, st_src, st_tgt, r_shared)
+    _geno tid RR geno f_src f_tgt r_ctx (o, trigger (Put st) >>= ktr_src) itr_tgt (ths, im_src, im_tgt, st_src, st_tgt, r_shared)
   | geno_getL
       f_src f_tgt r_ctx o
       ths im_src im_tgt st_src st_tgt r_shared
       ktr_src itr_tgt
-      (GENO: geno RR true f_tgt r_ctx (o, ktr_src st_src) itr_tgt (ths, im_src, im_tgt, st_src, st_tgt, r_shared))
+      (GENO: geno true f_tgt r_ctx (o, ktr_src st_src) itr_tgt (ths, im_src, im_tgt, st_src, st_tgt, r_shared))
     :
-    _geno tid geno RR f_src f_tgt r_ctx (o, trigger (@Get _) >>= ktr_src) itr_tgt (ths, im_src, im_tgt, st_src, st_tgt, r_shared)
+    _geno tid RR geno f_src f_tgt r_ctx (o, trigger (@Get _) >>= ktr_src) itr_tgt (ths, im_src, im_tgt, st_src, st_tgt, r_shared)
   | geno_tidL
       f_src f_tgt r_ctx o
       ths im_src im_tgt st_src st_tgt r_shared
       ktr_src itr_tgt
-      (GENO: geno RR true f_tgt r_ctx (o, ktr_src tid) itr_tgt (ths, im_src, im_tgt, st_src, st_tgt, r_shared))
+      (GENO: geno true f_tgt r_ctx (o, ktr_src tid) itr_tgt (ths, im_src, im_tgt, st_src, st_tgt, r_shared))
     :
-    _geno tid geno RR f_src f_tgt r_ctx (o, trigger (GetTid) >>= ktr_src) itr_tgt (ths, im_src, im_tgt, st_src, st_tgt, r_shared)
+    _geno tid RR geno f_src f_tgt r_ctx (o, trigger (GetTid) >>= ktr_src) itr_tgt (ths, im_src, im_tgt, st_src, st_tgt, r_shared)
   | geno_UB
       f_src f_tgt r_ctx o
       ths im_src im_tgt st_src st_tgt r_shared
       ktr_src itr_tgt
     :
-    _geno tid geno RR f_src f_tgt r_ctx (o, trigger (Undefined) >>= ktr_src) itr_tgt (ths, im_src, im_tgt, st_src, st_tgt, r_shared)
+    _geno tid RR geno f_src f_tgt r_ctx (o, trigger (Undefined) >>= ktr_src) itr_tgt (ths, im_src, im_tgt, st_src, st_tgt, r_shared)
   | geno_fairL
       f_src f_tgt r_ctx o
       ths im_src0 im_tgt st_src st_tgt r_shared
       f ktr_src itr_tgt
       (GENO: exists im_src1,
              (<<FAIR: fair_update im_src0 im_src1 (sum_fmap_r f)>>) /\
-               (<<GENO: geno RR true f_tgt r_ctx (o, ktr_src tt) itr_tgt (ths, im_src1, im_tgt, st_src, st_tgt, r_shared)>>))
+               (<<GENO: geno true f_tgt r_ctx (o, ktr_src tt) itr_tgt (ths, im_src1, im_tgt, st_src, st_tgt, r_shared)>>))
     :
-    _geno tid geno RR f_src f_tgt r_ctx (o, trigger (Fair f) >>= ktr_src) itr_tgt (ths, im_src0, im_tgt, st_src, st_tgt, r_shared)
+    _geno tid RR geno f_src f_tgt r_ctx (o, trigger (Fair f) >>= ktr_src) itr_tgt (ths, im_src0, im_tgt, st_src, st_tgt, r_shared)
 
   | geno_tauR
       f_src f_tgt r_ctx o
       ths im_src im_tgt st_src st_tgt r_shared
       itr_src itr_tgt
-      (GENO: geno RR f_src true r_ctx (o, itr_src) itr_tgt (ths, im_src, im_tgt, st_src, st_tgt, r_shared))
+      (GENO: geno f_src true r_ctx (o, itr_src) itr_tgt (ths, im_src, im_tgt, st_src, st_tgt, r_shared))
     :
-    _geno tid geno RR f_src f_tgt r_ctx (o, itr_src) (Tau itr_tgt) (ths, im_src, im_tgt, st_src, st_tgt, r_shared)
+    _geno tid RR geno f_src f_tgt r_ctx (o, itr_src) (Tau itr_tgt) (ths, im_src, im_tgt, st_src, st_tgt, r_shared)
   | geno_chooseR
       f_src f_tgt r_ctx o
       ths im_src im_tgt st_src st_tgt r_shared
       X itr_src ktr_tgt
-      (GENO: forall x, geno RR f_src true r_ctx (o, itr_src) (ktr_tgt x) (ths, im_src, im_tgt, st_src, st_tgt, r_shared))
+      (GENO: forall x, geno f_src true r_ctx (o, itr_src) (ktr_tgt x) (ths, im_src, im_tgt, st_src, st_tgt, r_shared))
     :
-    _geno tid geno RR f_src f_tgt r_ctx (o, itr_src) (trigger (Choose X) >>= ktr_tgt) (ths, im_src, im_tgt, st_src, st_tgt, r_shared)
+    _geno tid RR geno f_src f_tgt r_ctx (o, itr_src) (trigger (Choose X) >>= ktr_tgt) (ths, im_src, im_tgt, st_src, st_tgt, r_shared)
   | geno_putR
       f_src f_tgt r_ctx o
       ths im_src im_tgt st_src st_tgt r_shared
       st itr_src ktr_tgt
-      (GENO: geno RR f_src true r_ctx (o, itr_src) (ktr_tgt tt) (ths, im_src, im_tgt, st_src, st, r_shared))
+      (GENO: geno f_src true r_ctx (o, itr_src) (ktr_tgt tt) (ths, im_src, im_tgt, st_src, st, r_shared))
     :
-    _geno tid geno RR f_src f_tgt r_ctx (o, itr_src) (trigger (Put st) >>= ktr_tgt) (ths, im_src, im_tgt, st_src, st_tgt, r_shared)
+    _geno tid RR geno f_src f_tgt r_ctx (o, itr_src) (trigger (Put st) >>= ktr_tgt) (ths, im_src, im_tgt, st_src, st_tgt, r_shared)
   | geno_getR
       f_src f_tgt r_ctx o
       ths im_src im_tgt st_src st_tgt r_shared
       itr_src ktr_tgt
-      (GENO: geno RR f_src true r_ctx (o, itr_src) (ktr_tgt st_tgt) (ths, im_src, im_tgt, st_src, st_tgt, r_shared))
+      (GENO: geno f_src true r_ctx (o, itr_src) (ktr_tgt st_tgt) (ths, im_src, im_tgt, st_src, st_tgt, r_shared))
     :
-    _geno tid geno RR f_src f_tgt r_ctx (o, itr_src) (trigger (@Get _) >>= ktr_tgt) (ths, im_src, im_tgt, st_src, st_tgt, r_shared)
+    _geno tid RR geno f_src f_tgt r_ctx (o, itr_src) (trigger (@Get _) >>= ktr_tgt) (ths, im_src, im_tgt, st_src, st_tgt, r_shared)
   | geno_tidR
       f_src f_tgt r_ctx o
       ths im_src im_tgt st_src st_tgt r_shared
       itr_src ktr_tgt
-      (GENO: geno RR f_src true r_ctx (o, itr_src) (ktr_tgt tid) (ths, im_src, im_tgt, st_src, st_tgt, r_shared))
+      (GENO: geno f_src true r_ctx (o, itr_src) (ktr_tgt tid) (ths, im_src, im_tgt, st_src, st_tgt, r_shared))
     :
-    _geno tid geno RR f_src f_tgt r_ctx (o, itr_src) (trigger (GetTid) >>= ktr_tgt) (ths, im_src, im_tgt, st_src, st_tgt, r_shared)
+    _geno tid RR geno f_src f_tgt r_ctx (o, itr_src) (trigger (GetTid) >>= ktr_tgt) (ths, im_src, im_tgt, st_src, st_tgt, r_shared)
   | geno_fairR
       f_src f_tgt r_ctx o
       ths im_src im_tgt0 st_src st_tgt r_shared
       f itr_src ktr_tgt
       (GENO: forall im_tgt1
                    (FAIR: fair_update im_tgt0 im_tgt1 (sum_fmap_r f)),
-          (<<GENO: geno RR f_src true r_ctx (o, itr_src) (ktr_tgt tt) (ths, im_src, im_tgt1, st_src, st_tgt, r_shared)>>))
+          (<<GENO: geno f_src true r_ctx (o, itr_src) (ktr_tgt tt) (ths, im_src, im_tgt1, st_src, st_tgt, r_shared)>>))
     :
-    _geno tid geno RR f_src f_tgt r_ctx (o, itr_src) (trigger (Fair f) >>= ktr_tgt) (ths, im_src, im_tgt0, st_src, st_tgt, r_shared)
+    _geno tid RR geno f_src f_tgt r_ctx (o, itr_src) (trigger (Fair f) >>= ktr_tgt) (ths, im_src, im_tgt0, st_src, st_tgt, r_shared)
 
   | geno_observe
       f_src f_tgt r_ctx o
       ths im_src im_tgt st_src st_tgt r_shared
       fn args ktr_src ktr_tgt
       (GENO: forall ret,
-             geno RR true true r_ctx (o, ktr_src ret) (ktr_tgt ret) (ths, im_src, im_tgt, st_src, st_tgt, r_shared))
+             geno true true r_ctx (o, ktr_src ret) (ktr_tgt ret) (ths, im_src, im_tgt, st_src, st_tgt, r_shared))
     :
-    _geno tid geno RR f_src f_tgt r_ctx (o, trigger (Observe fn args) >>= ktr_src) (trigger (Observe fn args) >>= ktr_tgt) (ths, im_src, im_tgt, st_src, st_tgt, r_shared)
+    _geno tid RR geno f_src f_tgt r_ctx (o, trigger (Observe fn args) >>= ktr_src) (trigger (Observe fn args) >>= ktr_tgt) (ths, im_src, im_tgt, st_src, st_tgt, r_shared)
 
   | geno_yieldR
       f_src f_tgt r_ctx0 o0
@@ -180,10 +179,10 @@ Section GENORDER.
                im_tgt2
                (TGT: fair_update im_tgt1 im_tgt2 (sum_fmap_l (tids_fmap tid ths1))),
         exists o1,
-          (<<GENO: geno RR f_src true r_ctx1 (o1, trigger (Yield) >>= ktr_src) (ktr_tgt tt) (ths1, im_src1, im_tgt2, st_src1, st_tgt1, r_shared1)>>) /\
+          (<<GENO: geno f_src true r_ctx1 (o1, trigger (Yield) >>= ktr_src) (ktr_tgt tt) (ths1, im_src1, im_tgt2, st_src1, st_tgt1, r_shared1)>>) /\
             (<<STUTTER: wf_stt.(lt) o1 o0>>))
     :
-    _geno tid geno RR f_src f_tgt r_ctx0 (o0, trigger (Yield) >>= ktr_src) (trigger (Yield) >>= ktr_tgt) (ths0, im_src0, im_tgt0, st_src0, st_tgt0, r_shared0)
+    _geno tid RR geno f_src f_tgt r_ctx0 (o0, trigger (Yield) >>= ktr_src) (trigger (Yield) >>= ktr_tgt) (ths0, im_src0, im_tgt0, st_src0, st_tgt0, r_shared0)
 
   | geno_yieldL
       f_src f_tgt r_ctx o0
@@ -191,9 +190,9 @@ Section GENORDER.
       ktr_src itr_tgt
       (GENO: exists im_src1 o1,
           (<<FAIR: fair_update im_src0 im_src1 (sum_fmap_l (tids_fmap tid ths))>>) /\
-            (<<GENO: geno RR true f_tgt r_ctx (o1, ktr_src tt) itr_tgt (ths, im_src1, im_tgt, st_src, st_tgt, r_shared)>>))
+            (<<GENO: geno true f_tgt r_ctx (o1, ktr_src tt) itr_tgt (ths, im_src1, im_tgt, st_src, st_tgt, r_shared)>>))
     :
-    _geno tid geno RR f_src f_tgt r_ctx (o0, trigger (Yield) >>= ktr_src) itr_tgt (ths, im_src0, im_tgt, st_src, st_tgt, r_shared)
+    _geno tid RR geno f_src f_tgt r_ctx (o0, trigger (Yield) >>= ktr_src) itr_tgt (ths, im_src0, im_tgt, st_src, st_tgt, r_shared)
 
   | geno_progress
       r_ctx o
@@ -201,15 +200,15 @@ Section GENORDER.
       itr_src itr_tgt
       (GENO: ModSimNoSync.lsim I tid RR false false r_ctx itr_src itr_tgt (ths, im_src, im_tgt, st_src, st_tgt, r_shared))
     :
-    _geno tid geno RR true true r_ctx (o, itr_src) itr_tgt (ths, im_src, im_tgt, st_src, st_tgt, r_shared)
+    _geno tid RR geno true true r_ctx (o, itr_src) itr_tgt (ths, im_src, im_tgt, st_src, st_tgt, r_shared)
   .
 
   Definition geno (tid: thread_id)
              R_src R_tgt (RR: R_src -> R_tgt -> URA.car -> shared_rel):
     bool -> bool -> URA.car -> (wf_stt.(T) * itree srcE R_src) -> itree tgtE R_tgt -> shared_rel :=
-    pind7 (@_geno tid R_src R_tgt) top7 RR.
+    pind6 (_geno tid RR) top6.
 
-  Lemma geno_mon tid R0 R1: monotone7 (@_geno tid R0 R1).
+  Lemma geno_mon tid R0 R1 (RR: R0 -> R1 -> URA.car -> shared_rel): monotone6 (_geno tid RR).
   Proof.
     ii. inv IN; try (econs; eauto; fail).
     { des. econs; eauto. }
@@ -233,72 +232,72 @@ Section GENORDER.
   Proof.
     remember (o0, src) as osrc.
     move GENO before tid. revert_until GENO.
-    pattern LRR, ps, pt, r_ctx, osrc, tgt, shr.
-    revert LRR ps pt r_ctx osrc tgt shr GENO. apply pind7_acc.
-    intros rr DEC IH. clear DEC. intros LRR ps pt r_ctx osrc tgt shr GENO.
+    pattern ps, pt, r_ctx, osrc, tgt, shr.
+    revert ps pt r_ctx osrc tgt shr GENO. apply pind6_acc.
+    intros rr DEC IH. clear DEC. intros ps pt r_ctx osrc tgt shr GENO.
     i; clarify.
-    eapply pind7_unfold in GENO; eauto with paco.
+    eapply pind6_unfold in GENO; eauto with paco.
     inv GENO.
 
-    { eapply pind7_fold. econs 1; eauto. }
-    { eapply pind7_fold. econs 2; eauto.
+    { eapply pind6_fold. econs 1; eauto. }
+    { eapply pind6_fold. econs 2; eauto.
       destruct GENO0 as [GENO IND]. eapply IH in IND; eauto. split; ss.
     }
-    { eapply pind7_fold. econs 3; eauto.
+    { eapply pind6_fold. econs 3; eauto.
       des. destruct GENO0 as [GENO IND]. eapply IH in IND; eauto. esplits; eauto.
       split; ss; eauto.
     }
-    { eapply pind7_fold. econs 4; eauto.
+    { eapply pind6_fold. econs 4; eauto.
       destruct GENO0 as [GENO IND]. eapply IH in IND; eauto. split; ss.
     }
-    { eapply pind7_fold. econs 5; eauto.
+    { eapply pind6_fold. econs 5; eauto.
       destruct GENO0 as [GENO IND]. eapply IH in IND; eauto. split; ss.
     }
-    { eapply pind7_fold. econs 6; eauto.
+    { eapply pind6_fold. econs 6; eauto.
       destruct GENO0 as [GENO IND]. eapply IH in IND; eauto. split; ss.
     }
-    { eapply pind7_fold. econs 7; eauto. }
-    { eapply pind7_fold. econs 8; eauto.
+    { eapply pind6_fold. econs 7; eauto. }
+    { eapply pind6_fold. econs 8; eauto.
       des. destruct GENO as [GENO IND]. eapply IH in IND; eauto. esplits; eauto.
       split; ss; eauto.
     }
 
-    { eapply pind7_fold. econs 9; eauto.
+    { eapply pind6_fold. econs 9; eauto.
       destruct GENO0 as [GENO IND]. eapply IH in IND; eauto. split; ss.
     }
-    { eapply pind7_fold. econs 10; eauto.
+    { eapply pind6_fold. econs 10; eauto.
       i. specialize (GENO0 x).
       destruct GENO0 as [GENO IND]. eapply IH in IND; eauto. split; ss.
     }
-    { eapply pind7_fold. econs 11; eauto.
+    { eapply pind6_fold. econs 11; eauto.
       destruct GENO0 as [GENO IND]. eapply IH in IND; eauto. split; ss.
     }
-    { eapply pind7_fold. econs 12; eauto.
+    { eapply pind6_fold. econs 12; eauto.
       destruct GENO0 as [GENO IND]. eapply IH in IND; eauto. split; ss.
     }
-    { eapply pind7_fold. econs 13; eauto.
+    { eapply pind6_fold. econs 13; eauto.
       destruct GENO0 as [GENO IND]. eapply IH in IND; eauto. split; ss.
     }
-    { eapply pind7_fold. econs 14; eauto.
+    { eapply pind6_fold. econs 14; eauto.
       i. specialize (GENO0 _ FAIR).
       destruct GENO0 as [GENO IND]. eapply IH in IND; eauto. split; ss.
     }
-    { eapply pind7_fold. econs 15; eauto.
+    { eapply pind6_fold. econs 15; eauto.
       i. specialize (GENO0 ret).
       destruct GENO0 as [GENO IND]. eapply IH in IND; eauto. split; ss.
     }
 
-    { eapply pind7_fold. econs 16; eauto.
+    { eapply pind6_fold. econs 16; eauto.
       i. specialize (GENO0 _ _ _ _ _ _ _ INV0 VALID0 _ TGT). des. esplits; eauto.
       destruct GENO as [GENO IND]. eapply IH in IND; eauto. split; ss.
     }
 
-    { eapply pind7_fold. econs 17; eauto.
+    { eapply pind6_fold. econs 17; eauto.
       des. esplits; eauto.
-      eapply upind7_mon; eauto. ss.
+      eapply upind6_mon; eauto. ss.
     }
 
-    { eapply pind7_fold. econs 18; eauto. }
+    { eapply pind6_fold. econs 18; eauto. }
 
   Qed.
 
@@ -317,32 +316,32 @@ Section GENORDER.
     set (fzero:= fun _: (A R0 R1) => @ord_tree_base (A R0 R1)). set (one:= ord_tree_cons fzero).
     inv LSIM.
 
-    { exists one. eapply pind7_fold. econs 1; eauto.
+    { exists one. eapply pind6_fold. econs 1; eauto.
       instantiate (1:=fzero (ps, pt, r_ctx, Ret r_src, Ret r_tgt, (ths, im_src, im_tgt, st_src, st_tgt, r_shared))); ss.
     }
 
     { destruct LSIM0 as [LSIM IND]. eapply IH in IND. des.
-      exists o. eapply pind7_fold. econs 2; eauto. split; ss.
+      exists o. eapply pind6_fold. econs 2; eauto. split; ss.
     }
     { des. destruct LSIM0 as [LSIM IND]. eapply IH in IND. des.
-      exists o. eapply pind7_fold. econs 3; eauto. eexists. split; ss. eauto.
+      exists o. eapply pind6_fold. econs 3; eauto. eexists. split; ss. eauto.
     }
     { destruct LSIM0 as [LSIM IND]. eapply IH in IND. des.
-      exists o. eapply pind7_fold. econs 4; eauto. split; ss.
+      exists o. eapply pind6_fold. econs 4; eauto. split; ss.
     }
     { destruct LSIM0 as [LSIM IND]. eapply IH in IND. des.
-      exists o. eapply pind7_fold. econs 5; auto. split; ss.
+      exists o. eapply pind6_fold. econs 5; auto. split; ss.
     }
     { destruct LSIM0 as [LSIM IND]. eapply IH in IND. des.
-      exists o. eapply pind7_fold. econs 6; auto. split; ss.
+      exists o. eapply pind6_fold. econs 6; auto. split; ss.
     }
-    { exists one. eapply pind7_fold. econs 7; eauto. }
+    { exists one. eapply pind6_fold. econs 7; eauto. }
     { des. destruct LSIM as [LSIM IND]. eapply IH in IND. des.
-      exists o. eapply pind7_fold. econs 8; eauto. esplits; eauto. split; ss.
+      exists o. eapply pind6_fold. econs 8; eauto. esplits; eauto. split; ss.
     }
 
     { destruct LSIM0 as [LSIM IND]. eapply IH in IND. des. exists o.
-      eapply pind7_fold. econs 9; eauto. ss.
+      eapply pind6_fold. econs 9; eauto. ss.
     }
 
     { hexploit ord_tree_join.
@@ -354,7 +353,7 @@ Section GENORDER.
         eauto.
       }
       intro JOIN. des. exists o1.
-      eapply pind7_fold. econs 10.
+      eapply pind6_fold. econs 10.
       i. specialize (LSIM0 x). destruct LSIM0 as [LSIM IND].
       specialize (JOIN (ps, true, r_ctx, src, (ktr_tgt x), (ths, im_src, im_tgt, st_src, st_tgt, r_shared))).
       destruct JOIN; auto. des. split; ss.
@@ -362,13 +361,13 @@ Section GENORDER.
     }
 
     { destruct LSIM0 as [LSIM IND]. eapply IH in IND. des. exists o.
-      eapply pind7_fold. econs 11; eauto. ss.
+      eapply pind6_fold. econs 11; eauto. ss.
     }
     { destruct LSIM0 as [LSIM IND]. eapply IH in IND. des. exists o.
-      eapply pind7_fold. econs 12; eauto. ss.
+      eapply pind6_fold. econs 12; eauto. ss.
     }
     { destruct LSIM0 as [LSIM IND]. eapply IH in IND. des. exists o.
-      eapply pind7_fold. econs 13; eauto. ss.
+      eapply pind6_fold. econs 13; eauto. ss.
     }
 
     { hexploit ord_tree_join.
@@ -380,7 +379,7 @@ Section GENORDER.
         eauto.
       }
       intro JOIN. des. exists o1.
-      eapply pind7_fold. econs 14.
+      eapply pind6_fold. econs 14.
       i. specialize (LSIM0 _ FAIR). destruct LSIM0 as [LSIM IND].
       specialize (JOIN (ps, true, r_ctx, src, (ktr_tgt ()), (ths, im_src, im_tgt1, st_src, st_tgt, r_shared))).
       destruct JOIN; auto. des. split; ss.
@@ -396,7 +395,7 @@ Section GENORDER.
         eauto.
       }
       intro JOIN. des. exists o1.
-      eapply pind7_fold. econs 15.
+      eapply pind6_fold. econs 15.
       i. specialize (LSIM0 ret). destruct LSIM0 as [LSIM IND].
       specialize (JOIN (true, true, r_ctx, ktr_src ret, ktr_tgt ret, (ths, im_src, im_tgt, st_src, st_tgt, r_shared))).
       destruct JOIN; auto. des. split; ss.
@@ -412,7 +411,7 @@ Section GENORDER.
         eauto.
       }
       intro JOIN. des. exists o1.
-      eapply pind7_fold. econs 16.
+      eapply pind6_fold. econs 16.
       1,2: eauto.
       i. specialize (LSIM0 _ _ _ _ _ _ _ INV0 VALID0 _ TGT). destruct LSIM0 as [LSIM IND].
       specialize (JOIN (ps, true, r_ctx1, (x <- trigger Yield;; ktr_src x), ktr_tgt (), (ths1, im_src1, im_tgt2, st_src1, st_tgt1, r_shared1))).
@@ -420,11 +419,11 @@ Section GENORDER.
     }
 
     { des. destruct LSIM as [LSIM IND]. eapply IH in IND. des. exists o.
-      eapply pind7_fold. econs 17; eauto. esplits; eauto.
+      eapply pind6_fold. econs 17; eauto. esplits; eauto.
       split; ss. eauto.
     }
 
-    { exists one. eapply pind7_fold. econs 18. pclearbot. auto. }
+    { exists one. eapply pind6_fold. econs 18. pclearbot. auto. }
 
   Qed.
 
@@ -492,14 +491,15 @@ Section PROOF.
   Proof.
     eapply nosync_geno in LSIM. des.
     exists (mk_o (@wf_ot R0 R1) o ps src).
-    revert_until R1. ginit. gcofix CIH; i.
+    ginit. eapply cpn6_wcompat. eapply lsim_mon.
+    revert_until LRR. gcofix CIH; i.
     remember (o, src) as osrc.
     move LSIM before CIH. revert_until LSIM.
-    pattern LRR, ps, pt, r_ctx, osrc, tgt, shr.
-    revert LRR ps pt r_ctx osrc tgt shr LSIM. apply pind7_acc.
-    intros rr DEC IH. clear DEC. intros LRR ps pt r_ctx osrc tgt shr LSIM.
+    pattern ps, pt, r_ctx, osrc, tgt, shr.
+    revert ps pt r_ctx osrc tgt shr LSIM. apply pind6_acc.
+    intros rr DEC IH. clear DEC. intros ps pt r_ctx osrc tgt shr LSIM.
     intros src o Eosrc. clarify.
-    eapply pind7_unfold in LSIM; eauto with paco.
+    eapply pind6_unfold in LSIM; eauto with paco.
     inv LSIM.
 
     { guclo lsim_indC_spec. econs 1; eauto.
@@ -596,7 +596,7 @@ Section PROOF.
     { eapply nosync_geno in GENO. des.
       guclo lsim_ord_weakC_spec. econs.
       instantiate (1:=mk_o (@wf_ot R0 R1) o0 false src).
-      gfinal. right. pfold. eapply pind9_fold. econs 18. right. eapply CIH. auto.
+      gfinal. right. pfold. eapply pind6_fold. econs 18. right. eapply CIH. auto.
       ss. des_ifs; try reflexivity. right. ss. do 2 econs.
     }
 
